## Tabel 5


\(v=\left(\frac{\Delta x}{\Delta t}\right)_{\text {raaklijn }}\)
 \quad v=x^{\prime}\)
\(a_{\mathrm{gem}}=\frac{\Delta v}{\Lambda t}\)
\(a=v^{\prime}=x^{\prime}\)
\(x_{(t)}=x_{0}+v_{0} t+\frac{1}{2} a t^{2}\)
\(v_{(t)}=v_{0}+a t\)
\(s=\varphi r\)
\(\varphi \text { in rad }\)
\(\varphi=\omega t\)
\(\omega=\frac{v}{r}=\frac{2 \pi}{T}=2 \pi f\)
\(v=\frac{2 \pi r}{T} \quad v=\omega r=2 \pi f r\)
\(a_{\mathrm{mpz}}=\omega^{2} r=\frac{v^{2}}{r}=\omega v\)
\(F_{\mathrm{mpz}}=\frac{m v^{2}}{r}\)
\(F_{\mathrm{mpz}}=m \omega^{2} r=m \omega v\)
\(\vec{F}_{\mathrm{res}}=\sum \vec{F}_{\mathrm{i}}\)
\(F_{\mathrm{res}}=m a\)
\(\vec{F}_{\mathrm{AB}}=-\vec{F}_{\mathrm{BA}}\)
\(F_{\mathrm{z}}=m g\)
\(\vec{F}_{\mathrm{z}}=m \vec{g}\)
\(F_{\mathrm{w}, s, \max }=f F_{\mathrm{n}}\)
\(F_{\mathrm{w}, 1}=\frac{1}{2} \rho C_{\mathrm{w}} A v^{2}\)
\(F_{\mathrm{v}}=C u\)
\(p=m v\)
\(\Sigma \vec{p}_{\text {voor }}=\Sigma \vec{p}_{\mathrm{na}}\)
\(F=\frac{\mathrm{d} p}{\mathrm{~d} t}\)
\(\vec{S}=\vec{F} \Delta t=m \overrightarrow{\Delta v}=\overrightarrow{\Delta \dot{p}}\)
\(W=F s\)
\(W=F s \cos \alpha\)
\(W=\int F_{s} \mathrm{~d} s\)
\(E_{\mathrm{k}}=\frac{1}{2} m v^{2}\)
\(E_{\mathrm{z}}=m g h\)
\(E_{\mathrm{v}}=\frac{1}{2} C u^{2}\)
\(W_{\text {tot }}=\Delta E_{\mathrm{k}}\)
\(\Sigma W=\Delta E_{\mathrm{k}}\)
\(E_{\mathrm{tot}, \mathrm{in}}=E_{\mathrm{tot}, \mathrm{uit}}\)
\(\Sigma E_{\mathrm{in}}=\sum E_{\mathrm{uit}}\)
\(E_{\mathrm{ch}}=r_{V} V \)
\(E_{\mathrm{ch}}=r_{m} m\)
\(\eta=\frac{E_{\text {nuttig }}}{E_{\text {in }}}=\frac{P_{\text {nuttig }}}{P_{\text {in }}}\)
\(P=\frac{1}{2} \rho A v^{3}\)
\(F_{\mathrm{g}}=G \frac{m M}{r^{2}}\)
\(E_{\mathrm{g}}=-G \frac{m M}{r}\)
\(\omega r^{2}=\text { constant }\)
\(\frac{r^{3}}{T^{2}}=\frac{G M}{4 \pi^{2}}\)
\(I=\sum_{i} m_{i} r_{i}^{2}\)
\(I=m R^{2}\)
\(I=\frac{1}{2} m R^{2}\)
\(I=\frac{2}{3} m R^{2}\)
\(I=\frac{2}{5} m R^{2}\)
\(I=\frac{1}{4} m R^{2}\)
\(I=\frac{1}{12} m l^{2}\)
\(I=\frac{1}{3} m l^{2}\)
\(L=I \omega\)
\(L=m v_{\perp} r\)
\(M=I \alpha\)
\(E=\frac{1}{2} I \omega^{2}\)
\(\kappa=\frac{M}{\varphi}\)
\(f=\frac{1}{T}\)
\(\Delta \varphi=\frac{\Delta t}{T}\)
\(u=A \sin \left(\frac{2 \pi}{T} t\right)\)
\(v_{\max }=\frac{2 \pi A}{T}\)
\(\vec{F}_{\mathrm{res}}=-\overrightarrow{C u}\)
\(u_{(i)}=A \mathrm{e}^{-\delta t} \sin (2 \pi f t)\)
\(T=2 \pi \sqrt{\frac{m}{C}}\)
\(T=2 \pi \sqrt{\frac{l}{g}}\)
\(T=2 \pi \sqrt{\frac{I}{m g l}}\)
\(T=2 \pi \sqrt{\frac{I}{\kappa}}\)
\(v=\frac{\lambda}{T}\)
\(v=\sqrt{\frac{F_{s} l}{m}}\)
\(v=\sqrt{g h}\)
\(v=\sqrt{\frac{E}{\rho}}\)
\(v=\sqrt{\frac{K}{\rho}}\)
\(v=\sqrt{\frac{C_{p}}{C_{V}} \frac{p}{\rho}}=\sqrt{\frac{C_{p}}{C_{V}} \frac{R T}{M}}\)
\(l=n \frac{1}{2} \lambda\)
\(l=(2 n-1) \frac{1}{4} \lambda\)
\(\frac{\sin i}{\sin r}=\frac{v_{1}}{v_{2}}=n_{1 \rightarrow 2}\)
\(f_{\mathrm{w}}=f_{\mathrm{b}} \frac{v-v_{\mathrm{w}}}{v-v_{\mathrm{b}}}\)
\(L_{p}=20 \log \frac{p}{p_{0}}\)
\(\mathrm{m}^{-2}  L_{I}=10 \log \frac{I}{I_{0}}\)
\(I=\frac{P_{\text {bron }}^{2}}{4 \pi r^{2}}\)
\(\angle i=\angle t\)
\(n_{1 \rightarrow 2}=\frac{n_{2}}{n_{1}}=\frac{c_{1}}{c_{2}}\)
\(\frac{\sin i}{\sin r}=n_{1 \rightarrow 2}\)
\(S=\frac{1}{b}+\frac{1}{v}=\frac{1}{f}\)
\(N_{\operatorname{lin}}=\mid \frac{b}{v}\)
\(\sin g=\frac{1}{n}\)
\(N_{\mathrm{ang}}=\frac{n}{f}\)
\(S=(n-1)\left(\frac{1}{r_{1}}-\frac{1}{r_{2}}\right)\)
\(S=S_{1}+S_{2}+\ldots\)
\(N_{\mathrm{ang}}=\frac{f_{\mathrm{obj}}}{f_{\mathrm{oc}}}\)
\(\frac{1}{b}+\frac{1}{v}=\frac{1}{f}=\frac{2}{R}\)
\(\sin \alpha_{n}=\frac{n \lambda}{d}\)
\(\sin \alpha_{n}=\frac{n \lambda}{d}\)
\(\cos \alpha_{n}=\frac{n \lambda}{2 d}\)
\(p=\frac{F}{A}\)
\(\rho=\frac{m}{V}\)
\(T_{\text {celsius }}=T_{\text {kelvin }}-273,15\)
\(l=l_{0}(1+\alpha \Delta \mathrm{T})\)
\(V=V_{0}(1+\gamma \Delta \mathrm{T})\)
\(\gamma=3 \alpha\)
\(p=\rho g h\)
\(p=\frac{1}{2} \rho v^{2}\)
\(F_{\text {opw }}=\rho g V\)
\(Q=\frac{\Delta V}{\Delta t}=A v\)
\(A v= constant\)
\(p+\frac{1}{2} \rho v^{2}+\rho g h= constant\)
\(F_{\mathrm{w}}=6 \pi \eta r v\)
\(Q=\frac{\Delta V}{\Delta t}=\frac{\pi r^{4}}{8 \eta l} \Delta p\)
\(p V=n R T\)
\(\left(p+\frac{n^{2} a}{V^{2}}\right)(V-n b)=n R T\)
\(V_{t}=V_{0}(1+\gamma \Delta T)\)
\(p_{t}=p_{0}(1+\gamma \Delta T)\)
\(M=N_{\mathrm{A}} m_{\text {molecuul }}\)
\(m=n M\)
\(p V^{\gamma}= constant \quad \gamma=\frac{c_{p}}{c_{V}}\)
\(\overline{|v|}=\sqrt{\frac{8 k T}{\pi m_{\mathrm{m}}}}\)
\(v_{\mathrm{w}}=\sqrt{\frac{2 k T}{m_{\mathrm{m}}}}\)
\(Q=c m \Delta T\)
\(c=\frac{C}{m}\)
\(c_{p}=\frac{Q_{p}}{m \Delta T}\)
\(c_{V}=\frac{Q_{V}}{m \Delta T}\)
\(r_{\mathrm{s}}=\frac{Q_{s}}{m}\)
\(r_{\mathrm{v}}=\frac{Q_{\mathrm{v}}}{m}\)
\(W_{\mathrm{u}}=p \Delta V\)
\(Q=\Delta E_{\mathrm{pot}}+\Delta E_{\mathrm{k}}+W_{\mathrm{u}}\)
\(\eta=\frac{W_{\mathrm{u}}}{Q}\)
\(\eta=\frac{Q_{1}-Q_{2}}{Q_{1}}=\frac{T_{1}-T_{2}}{T_{1}}\)
\(\eta=\frac{W_{\mathrm{u}}}{Q}<1\)
\(S=k \ln W\)
\(\Delta S=\int \frac{1}{T} \mathrm{~d} Q\)
\(P=\lambda A\)
\(P=\frac{\mathrm{d} Q}{\mathrm{~d} t}\)
\(I=\frac{Q}{t}\)
\(U=\frac{\Delta E}{Q}\)
\(U=I R\)
\(I=G U\)
\(G=\frac{1}{R}\)
\(I_{\mathrm{tot}}=I_{1}=I_{2}=\ldots\)
\(U_{\mathrm{tot}}=U_{1}+U_{2}+\ldots\)
\(R_{\text {tot }}=R_{1}+R_{2}+\ldots\)
\(\frac{1}{G_{\text {tot }}}=\frac{1}{G_{1}}+\frac{1}{G_{2}}+\ldots\)
\(I_{\mathrm{tot}}=I_{1}+I_{2}+\ldots\)
\(U_{\mathrm{tot}}=U_{1}=U_{2}=\ldots\)
\(G_{\mathrm{tot}}=G_{1}+G_{2}+\ldots\)
\(\frac{1}{R_{\text {tot }}}=\frac{1}{R_{1}}+\frac{1}{R_{2}}+\ldots\)
\(P=U I\)
\(E=P t\)
\(\rho=\frac{R A}{l}\)
\(R_{t}=R_{0}(1+\alpha \Delta T)\)
\(\sum_{i} I_{i}=0\)
\(\sum_{i} U_{i}=0\)
\(m=A I t=\frac{A_{\mathrm{r}}}{F v} I\)
\(F_{\mathrm{el}}=f \frac{q Q}{r^{2}}\)
\(f=\frac{1}{4 \pi \varepsilon_{\mathrm{r}} \varepsilon_{0}}\)
\(U_{\mathrm{el}}=-f \frac{Q}{r}\)
\(\vec{F}_{\mathrm{el}}=q \vec{E}\)
\(E=\frac{U}{\Delta x}\)
\(\Delta E_{\mathrm{el}}=q U\)
\(\Delta E_{\mathrm{k}}=-\Delta E_{\mathrm{el}}\)
\(W_{\mathrm{A} \rightarrow \mathrm{B}}=q U_{\mathrm{AB}}\)
\(C=\frac{Q}{U}\)
\(E=\frac{1}{2} C U^{2}\)
\(I_{(t)}=I_{0} \mathrm{e}^{-\frac{t}{R C}}\)
\(U_{\omega}=U_{\infty}\left(1-\mathrm{e}^{-\frac{t}{R C}}\right)\)
\(\frac{1}{C_{\text {tot }}}=\frac{1}{C_{1}}+\frac{1}{C_{2}}+\ldots\)
\(C_{\mathrm{tot}}=C_{1}+C_{2}+\ldots\)
\(F_{\mathrm{L}}=B I l\)
\(F_{\mathrm{L}}=B I l \sin \alpha\)
\(F_{\mathrm{L}}=B q v\)
\(F_{\mathrm{L}}=B q v \sin \alpha\)
\(\Phi=B_{\perp} A\)
\(\Phi=B A \cos \alpha\)
\(\mu=\mu_{0} \mu_{\mathrm{r}}\)
\(B=\mu \frac{I}{2 \pi r}\)
\(B=\mu \frac{N I}{l}\)
\(B=\mu \frac{N I}{l} \frac{l}{\sqrt{l^{2}+4 r^{2}}}\)
\(B_{\mathrm{as}}=\frac{1}{2} \mu \frac{r^{2} I}{\left(r^{2}+l^{2}\right)^{\frac{3}{2}}}\)
\(F=\frac{\mu_{0}}{2 \pi} \frac{I_{1} I_{2}}{r} l\)
\(U_{\text {ind }}=-N \frac{\mathrm{d} \Phi}{\mathrm{d} t}\)
\(U_{\text {zelind }}=-L \frac{\mathrm{d} I}{\mathrm{~d} t}\)
\(L=\mu \frac{N^{2} A}{l}\)
\(L_{\mathrm{tot}}=L_{1}+L_{2}+\ldots\)
\(\frac{1}{L_{\text {tot }}}=\frac{1}{L_{1}}+\frac{1}{L_{2}}+\ldots\)
\(E=\frac{1}{2} L I^{2}\)
\(I_{(t)}=I_{0} \mathrm{e}^{-\frac{R}{L} t}\)
\(C=\frac{\varepsilon A}{d}\)
\(U=U_{\max } \sin (2 \pi f t)\)
\(I=I_{\max } \sin (2 \pi f t)\)
\(U_{\mathrm{eff}}=\frac{1}{2} \sqrt{2} U_{\max }\)
\(I_{\mathrm{eff}}=\frac{1}{2} \sqrt{2} I_{\max }\)
\(P_{\mathrm{eff}}=U_{\mathrm{eff}} I_{\mathrm{eff}}=\frac{1}{2} P_{\max }\)
\(\frac{U_{\mathrm{p}}}{U_{\mathrm{s}}}=\frac{N_{\mathrm{p}}}{N_{\mathrm{s}}}\)
\(\frac{U_{\mathrm{p}}}{U_{\mathrm{s}}}=\frac{I_{\mathrm{s}}}{I_{\mathrm{p}}}\)
\(P_{\mathrm{p}}=P_{\mathrm{s}}\)
\(P_{\text {bron }}=\sigma A T^{4}\)
\(\lambda_{\max } T=k_{\mathrm{W}}\)
\(v=\frac{\Delta \lambda}{\lambda}\)
\(I_{(x)}\)
\(E_{\mathrm{f}}=h f\)
\(E_{\mathrm{f}}=\frac{h c}{\lambda}\)
\(c=f \lambda\)
\(E_{\mathrm{f}}=\left|E_{\mathrm{m}}-E_{\mathrm{n}}\right|\)
\(W=h f_{\mathrm{grens}}\)
\(E_{\mathrm{k}} \leq h f-W_{\mathrm{u}}\)
\(p=m c=\frac{h}{\lambda}\)
\(r_{\mathrm{n}}=\frac{\varepsilon_{0} h^{2}}{\pi e^{2} m_{\mathrm{e}}} n^{2}\)
\(E_{\mathrm{n}}=-\frac{13,6(\mathrm{ineV})}{n^{2}}\)
\(E_{\mathrm{n}}=-\frac{m e^{4}}{8 \varepsilon_{0}^{2} n^{2} h^{2}}\)
\(A=N+Z\)
\(E=m c^{2}\)
\(N=N_{0}\left(\frac{1}{2}\right)^{n}\)
\(n=\frac{t}{t_{\frac{1}{2}}} N=N_{0}\left(\frac{1}{2}\right)^{\frac{t}{t_{1}}}\)
\(A=-\left(\frac{\Delta N}{\Delta t}\right)_{\text {raaklijn }} \)
\( A=-\frac{\mathrm{d} N}{\mathrm{~d} t}\)
\(A_{\mathrm{gem}}=-\frac{\Delta N}{\Delta t} \)
\( A=\frac{\ln 2}{t_{\frac{1}{2}}} N\)
\(A=A_{0}\left(\frac{1}{2}\right)^{n} \)
\( n=\frac{t}{t_{\frac{1}{2}}} \)
\( A=A_{0}\left(\frac{1}{2}\right)^{\frac{t}{l_{\frac{1}{2}}}}\)
\(I=I_{0}\left(\frac{1}{2}\right)^{n} \)
\( n=\frac{d}{d_{\frac{1}{2}}} I=I_{0}\left(\frac{1}{2}\right)^{\frac{d}{d_{\frac{1}{2}}}}\)
\(\bar{E}=\frac{1}{3} E_{\max }\)
\(D=\frac{E}{m}\)
\(H=w_{\mathrm{R}} D\)
\(H_{\mathrm{eff}}=\sum w_{\mathrm{org}} H_{\mathrm{org}}\)
\(t_{\frac{1}{2}} \text { eff }=\frac{t_{\frac{1}{1}} \cdot t_{\frac{1}{2}} \text { biol }}{t_{\frac{1}{2}}+t_{\frac{1}{2}} \text { biol }}\)
\(\lambda=\frac{h}{p} \)
\( \lambda=\frac{h}{m_{0} v}\)
\(\Delta x \Delta p \geq \frac{h}{4 \pi}\)
\(E_{n}=\frac{n^{2} h^{2}}{8 m L^{2}}\)
\(\int_{-\infty}^{\infty}\left|\psi_{(\mathrm{x})}\right|^{2} \mathrm{~d} x=1 \frac{\mathrm{d}^{2} \psi}{\mathrm{d} x^{2}}+\frac{\mathrm{d}^{2} \psi}{\mathrm{d} y^{2}}+\frac{\mathrm{d}^{2} \psi}{\mathrm{d} z^{2}}=-\frac{8 \pi^{2} m}{h^{2}}\left(E+\frac{e^{2}}{4 \pi \varepsilon_{0} r}\right) \psi\)
\(v_{\mathrm{D}}=\frac{e U}{m_{\mathrm{e}} l} \tau\)
\(I=n e v_{\mathrm{D}} A\)
\(U_{\mathrm{H}}=B v_{\mathrm{D}} b\)
\(R=R_{0}(1+\alpha t)\)
\(R_{(T)}=C \mathrm{e}^{\frac{B}{T}}\)
\(\gamma=\frac{1}{\sqrt{1-\frac{v^{2}}{c^{2}}}}\)
\(\Delta t_{\mathrm{b}}=\frac{\Delta t_{\mathrm{e}}}{\sqrt{1-\frac{v^{2}}{c^{2}}}}=\gamma \Delta t_{\mathrm{e}}\)
\(l_{\mathrm{b}}=l_{\mathrm{c}} \sqrt{1-\frac{v^{2}}{c^{2}}}=\frac{l_{\mathrm{c}}}{\gamma}\)
\(w=\frac{u+v}{1+\frac{u v}{c^{2}}}\)
\(f_{b}=f_{e} \sqrt{\frac{c+v}{c-v}}\)
\(m=\frac{m_{0}}{\sqrt{1-\frac{v^{2}}{c^{2}}}}=\gamma m_{0}\)
\(E=\sqrt{m_{0}^{2} c^{4}+p^{2} c^{2}}\)
\(p_{(h)}=p_{0} \mathrm{e}^{-\frac{M_{\mathrm{r}} g h}{R T}}\)
\(\rho=\frac{p M}{R T}\)
\(e_{(T)}=\frac{p_{(T)}}{p_{\max (T)}}\)
\(h_{\mathrm{c}}=c_{1}\left(T-T_{\mathrm{d}}\right)\)
\(v=\frac{2 \rho g}{9 \eta} r^{2}\)
